Fix.

sample-bot.lean
@@ -1,11 +1,10 @@
 import ircbot
-open types effects
+open types effects support
 
 def server : string := "irc.mozilla.org"
 def port : string := "6667"
 
 def ident : string := "lean"
-
 def bot_nickname : string := "leanbot"
 
 theorem bot_nickname_is_correct : bot_nickname.front ≠ '#' :=
@@ -13,24 +12,15 @@ begin
   intros contra, cases contra
 end
 
-/-
-def wait (time : string) : io unit := do
-  wait_proc ← io.proc.spawn { cmd := "sleep",
-                              args := [time] },
-  io.proc.wait wait_proc,
-  pure ()
--/
-
-def join (input : irc_text) : list irc_text :=
+def join_at_start (input : irc_text) : list irc_text :=
 match input with
 | irc_text.parsed_normal v :=
   if v.type = message.mode ∧
      v.text = "+x" ∧
      v.subject = bot_nickname then
-    list.map irc_text.raw_text
-      ["JOIN #borsch\n",
-       "PRIVMSG #borsch I can not in fucking unicode!\n",
-       sformat! "MODE {bot_nickname} +B\n"]
+     [join "#borsch",
+      privmsg "#borsch" "Black magic is here!",
+      mode bot_nickname "+B"]
   else []
 | _ := []
 end
@@ -38,46 +28,35 @@ end
 def ping_pong (input : irc_text) : list irc_text :=
 match input with
 | irc_text.parsed_normal
-  { object := ~nick!ident, type := message.privmsg,
+  { object := some ~nick!ident, type := message.privmsg,
     subject := subject, text := "ping" } :=
-  [irc_text.parsed_normal
-    { object := person.unidentified bot_nickname,
-      type := message.privmsg,
-      subject :=
-        if subject.front = '#' then subject
-        else nick,
-      text := sformat! "{nick}, pong" }]
+  let new_subject :=
+    if subject.front = '#' then subject else nick in
+  [privmsg new_subject $ sformat! "{nick}, pong"]
 | _ := []
 end
 
 theorem ping_pong_is_correct_on_channel (nick ident subject: string)
   (on_channel : subject.front = '#') :
   (ping_pong $ irc_text.parsed_normal
-    { object := ~nick!ident,
+    { object := some ~nick!ident,
       type := message.privmsg,
       subject := subject,
       text := "ping" }) =
-  [irc_text.parsed_normal
-    { object := person.unidentified bot_nickname,
-      type := message.privmsg,
-      subject := subject,
-      text := sformat! "{nick}, pong" }] := begin
+  [privmsg subject $ sformat! "{nick}, pong"] := begin
   intros, simp [ping_pong], rw [on_channel], trivial
 end
 
 theorem ping_pong_is_correct_on_priv (nick ident subject: string)
   (not_on_channel : subject = bot_nickname):
   (ping_pong $ irc_text.parsed_normal
-    { object := ~nick!ident,
+    { object := some ~nick!ident,
       type := message.privmsg,
       subject := bot_nickname,
       text := "ping" }) =
-  [irc_text.parsed_normal
-    { object := person.unidentified bot_nickname,
-      type := message.privmsg,
-      subject := nick,
-      text := sformat! "{nick}, pong" }] := begin
-  intros, simp [ping_pong], simp [bot_nickname_is_correct]
+  [privmsg nick $ sformat! "{nick}, pong"] := begin
+  intros, simp [privmsg], simp [ping_pong],
+  simp [privmsg], simp [bot_nickname_is_correct]
 end
 
 def my_bot : bot :=
@@ -85,6 +64,6 @@ def my_bot : bot :=
   ident := ident,
   server := server,
   port := port,
-  funcs := [join, ping_pong] }
+  funcs := [join_at_start, ping_pong] }
 
 def main := mk_bot my_bot
