ircbot/default.lean
@@ -1,1 +1,1 @@
-import ircbot.types ircbot.effects
+import ircbot.types ircbot.effects ircbot.support
